cleaning

foterms_std.v
@@ -1,6 +1,6 @@
 (* First-Order Terms with no Eigen Variable *)
 
-Require Export foterms.
+From Quantifiers Require Export foterms.
 
 Set Implicit Arguments.
 
@@ -13,19 +13,16 @@ Notation "r ;; s" := (fecomp r s) (at level 20, format "r  ;;  s").
 Notation closed t := (tvars t = nil).
 Notation fclosed r := (forall n, closed (r n)).
 
-Arguments tvar {_} {_} {T} _.
-
 (* Function allowing to embed [term Empty_set] into any [term T]
      through identity embedding by using [tesubs (r_empty T)] *)
-Definition r_empty T : Empty_set -> @term vatom tatom T :=
-  fun z => match z with end.
+Definition r_empty T : Empty_set -> @term vatom tatom T := fun z => match z with end.
 
 Lemma fclosed_r_empty T : fclosed (r_empty T).
-Proof. intros n; destruct n. Qed.
+Proof. intros []. Qed.
 Hint Resolve fclosed_r_empty : term_db.
 
-Lemma fecomp_r_empty T1 T2 : forall s, r_empty T1 ;; s == r_empty T2.
-Proof. intros s n; destruct n. Qed.
+Lemma fecomp_r_empty T1 T2 s : r_empty T1 ;; s ~ r_empty T2.
+Proof. intros []. Qed.
 Hint Rewrite fecomp_r_empty : term_db.
 
 End Terms.
