foformulas_ar.v
@@ -2,7 +2,7 @@
 
 (* with arity checks *)
 
-Require Export foterms_ar.
+From Quantifiers Require Export foterms_ar.
 
 Set Implicit Arguments.
 
@@ -130,8 +130,7 @@ Proof. formula_induction A. Qed.
 Hint Rewrite esubs_comp : term_db.
 
 (* the result of substitution depends extensionnaly on the substituting function *)
-Lemma esubs_ext T1 T2 k (r1 r2 : T1 -> term T2 0) :
-  r1 == r2 -> forall A : formula T1 k, A⟦r1⟧ = A⟦r2⟧.
+Lemma esubs_ext T1 T2 k (r1 r2 : T1 -> term T2 0) : r1 ~ r2 -> forall A : formula T1 k, A⟦r1⟧ = A⟦r2⟧.
 Proof. formula_induction A. Qed.
 
 
