foterms_vec.v
@@ -6,15 +6,15 @@
 From Coq Require Export PeanoNat.
 From Coq Require Vector.
 From OLlibs Require Export dectype List_more.
-
-Require Export term_tactics.
+From Quantifiers Require Export term_tactics.
 
 Set Implicit Arguments.
 
 Notation vec := Vector.t.
 
 (* Extensional equality of functions *)
-Infix "==" := (fun f g => forall x, f x = g x) (at level 70).
+Definition ext_eq {A B} (f g : A -> B) := (forall a, f a = g a).
+Notation " f ~ g " := (ext_eq f g) (at level 60).
 
 
 (** * First-Order Terms *)
@@ -110,14 +110,12 @@ Hint Rewrite tesubs_evar : term_db.
 Definition fecomp T1 T2 T3 (r : T1 -> term T2) (s : T2 -> term T3) := fun x => (r x)⟦s⟧.
 Notation "r ;; s" := (fecomp r s) (at level 20, format "r  ;;  s").
 
-Lemma tesubs_comp T1 T2 T3 (r : T1 -> term T2) (s : T2 -> term T3) :
-  forall t, t⟦r⟧⟦s⟧ = t⟦r ;; s⟧.
+Lemma tesubs_comp T1 T2 T3 (r : T1 -> term T2) (s : T2 -> term T3) t : t⟦r⟧⟦s⟧ = t⟦r ;; s⟧.
 Proof. term_induction t. Qed.
 Hint Rewrite tesubs_comp : term_db.
 
 (* the result of substitution depends extensionnaly on the substituting function *)
-Lemma tesubs_ext T1 T2 (r1 r2 : T1 -> term T2) :
-  r1 == r2 -> forall t, t⟦r1⟧ = t⟦r2⟧.
+Lemma tesubs_ext T1 T2 (r1 r2 : T1 -> term T2) : r1 ~ r2 -> forall t, t⟦r1⟧ = t⟦r2⟧.
 Proof. term_induction t. Qed.
 Hint Resolve tesubs_ext : term_db.
 (* TODO could be turned into a morphism *)
@@ -140,7 +138,7 @@ match t with
 end.
 Notation "t [ u // x ]" := (tsubs x u t) (at level 8, format "t [ u // x ]").
 
-Lemma tsubs_tsubs_eq : forall x u v t, t[v//x][u//x] = t[v[u//x]//x].
+Lemma tsubs_tsubs_eq x u v t : t[v//x][u//x] = t[v[u//x]//x].
 Proof. term_induction t. Qed.
 Hint Rewrite tsubs_tsubs_eq : term_db.
 
@@ -158,23 +156,22 @@ Notation "x ∉ t" := (~ In x (tvars t)) (at level 30).
 Notation closed t := (tvars t = nil).
 Notation fclosed r := (forall n, closed (r n)).
 
-Lemma closed_notvars : forall t x, closed t -> x ∉ t.
-Proof. intros t x Hc Hin ; now rewrite Hc in Hin. Qed.
+Lemma closed_notvars t x : closed t -> x ∉ t.
+Proof. intros Hc Hin. rewrite Hc in Hin. destruct Hin. Qed.
 Hint Resolve closed_notvars : term_db.
 
-Lemma tvars_tsubs_closed : forall x u, closed u -> forall t,
-  tvars t[u//x] = remove eq_dt_dec x (tvars t).
+Lemma tvars_tsubs_closed x u : closed u -> forall t, tvars t[u//x] = remove eq_dt_dec x (tvars t).
 Proof.
 term_induction t.
-rewrite remove_concat, flat_map_concat_map, ? Vector.to_list_map, ? map_map; f_equal.
+rewrite remove_concat, flat_map_concat_map, ? Vector.to_list_map, ? map_map. f_equal.
 apply Vector.to_list_Forall in IHl.
-apply map_ext_in; intros v Hv; now specialize_Forall IHl with v.
+apply map_ext_in. intros v Hv. now specialize_Forall IHl with v.
 Qed.
 Hint Rewrite tvars_tsubs_closed using intuition; fail : term_db.
 
-Lemma notin_tsubs : forall x u t, x ∉ t -> t[u//x] = t.
+Lemma notin_tsubs x u t : x ∉ t -> t[u//x] = t.
 Proof.
-term_induction t; try rcauto; f_equal.
+term_induction t; try rcauto.
 apply IHl; intros Hx; apply H.
 rewrite Vector.to_list_map, <- flat_map_concat_map.
 apply in_flat_map; exists i; intuition.
@@ -190,7 +187,7 @@ Proof. term_induction t. Qed.
 Hint Rewrite tsubs_tsubs using try (intuition; fail);
                               (try apply closed_notvars); intuition; fail : term_db.
 
-Lemma notin_tsubs_bivar : forall x y t, x ∉ t -> t[tvar x//y][tvar y//x] = t.
+Lemma notin_tsubs_bivar x y t : x ∉ t -> t[tvar x//y][tvar y//x] = t.
 Proof.
 term_induction t.
 apply IHl; intros Hx; apply H.
@@ -220,12 +217,11 @@ Hint Rewrite notin_tsubs using try easy;
 
 (** * Additional results with variable eigen type *)
 
-Lemma tvars_tesubs_fclosed : fclosed -> forall t, tvars t⟦r⟧ = tvars t.
+Lemma tvars_tesubs_fclosed t : fclosed -> tvars t⟦r⟧ = tvars t.
 Proof. term_induction t. Qed.
 Hint Rewrite tvars_tesubs_fclosed using intuition; fail : term_db.
 
-Lemma tsubs_tesubs : forall x u t, fclosed ->
-  t[u//x]⟦r⟧ = t⟦r⟧[u⟦r⟧//x].
+Lemma tsubs_tesubs x u t : fclosed -> t[u//x]⟦r⟧ = t⟦r⟧[u⟦r⟧//x].
 Proof. term_induction t. Qed.
 Hint Rewrite tsubs_tesubs using intuition; fail : term_db.
 
@@ -284,8 +280,8 @@ Lemma fclosed_fesubs : forall v, closed v -> fclosed (v⇓).
 Proof. intros v Hc n; now destruct n. Qed.
 Hint Resolve fclosed_fesubs : term_db.
 
-Lemma fesubs_fup v : ⇑ ;; v⇓ == evar.
-Proof. intros ?; reflexivity. Qed.
+Lemma fesubs_fup v : ⇑ ;; v⇓ ~ evar.
+Proof. intro. reflexivity. Qed.
 
 Lemma tesubs_fup v t : t↑⟦v⇓⟧ = t.
 Proof. rcauto. Qed.
@@ -300,14 +296,14 @@ Definition felift u r := fun n =>
 Notation "⇑[ u ] r" := (felift u r) (at level 25, format "⇑[ u ] r").
 
 Lemma fclosed_felift u r : closed u -> fclosed r -> fclosed (⇑[u]r).
-Proof. intros ? ? n; rnow destruct n. Qed.
+Proof. rnow intros ? ? [|]. Qed.
 Hint Resolve fclosed_felift : term_db.
 
-Lemma felift_comp u r : r ;; ⇑ == ⇑ ;; ⇑[u]r.
-Proof. intros ?; reflexivity. Qed.
+Lemma felift_comp u r : r ;; ⇑ ~ ⇑ ;; ⇑[u]r.
+Proof. intro. reflexivity. Qed.
 Hint Rewrite felift_comp : term_db.
 
-Lemma felift_tesubs u r : forall t, t⟦r⟧↑ = t↑⟦⇑[u]r⟧.
+Lemma felift_tesubs u r t : t⟦r⟧↑ = t↑⟦⇑[u]r⟧.
 Proof. rcauto. Qed.
 Hint Rewrite felift_tesubs : term_db.
 
