hilbert.v
@@ -1,8 +1,7 @@
 (* Hilbert system for Intuitionistic Logic with implication and quantifiers *)
 
 From Coq Require Import List.
-
-Require Import foformulas_ext.
+From Quantifiers Require Import foformulas_ext.
 
 Set Implicit Arguments.
 
