term_tactics.v
@@ -6,16 +6,16 @@ From OLlibs Require Import dectype.
 Create HintDb term_db.
 Ltac Tauto.intuition_solver ::= auto with datatypes term_db.
 
-Lemma ltb_S : forall n m, (S n <? S m) = (n <? m).
+Lemma ltb_S n m : (S n <? S m) = (n <? m).
 Proof. reflexivity. Qed.
 #[export] Hint Rewrite ltb_S : term_db.
 
 
 Tactic Notation "rnow" tactic(t) :=
-  t; ( try now autorewrite with term_db in * ); (* intuition may do too many intros *)
+  t; try (now autorewrite with term_db in *); (* intuition may do too many intros *)
      simpl; autorewrite with term_db in *; cbn; intuition.
 Tactic Notation "rnow" tactic(t) "then" tactic(t1) :=
-  t; ( try now autorewrite with term_db in * ); (* intuition may do too many intros *)
+  t; try (now autorewrite with term_db in *); (* intuition may do too many intros *)
      simpl; autorewrite with term_db in *; cbn; intuition t1; simpl; intuition.
 
 Ltac rcauto := simpl; intuition; autorewrite with term_db in *; simpl; rnow (repeat case_analysis).
